From OEIS, note that this is not Central factorial number itself, this formula is in the mathematica package as
\texttt{OEISFormula}
\begin{equation*}
    T_{\mathrm{OEIS}} (n,k) = \frac{1}{m} \sum_{j=0}^{m} (-1)^{j} \binom{2m}{j} (m-j)^{2n}
\end{equation*}
where $m=n-k+1$.
So that
\begin{equation*}
    T_{\mathrm{OEIS}} = \frac{1}{n-k+1} \sum_{j=0}^{n-k+1} (-1)^{j} \binom{2n-2k+2}{j} (n-k+1-j)^{2n}
\end{equation*}
Also, OEIS sequence is defined by
\begin{equation*}
    T_{\mathrm{OEIS}} = (2(n-k) + 1)! T(2n, 2n-2k)
\end{equation*}
where $T(2n, 2n-2k)$ are central factorial numbers.
From stackoverflow, these are pure central factorial numbers already
\begin{equation*}
    k! T(n,k) = \sum_{j=0} \binom{k}{j} (-1)^{j} \left( \frac{1}{2}k - j \right)^{n}
\end{equation*}
So that central factorial number is, this is the function \texttt{Central1(n,k)} in mathematica package
\begin{equation*}
    T(n,k) = \frac{1}{k!} \sum_{j=0} \binom{k}{j} (-1)^{j} \left( \frac{1}{2}k - j \right)^{n}
\end{equation*}
Let be $(k-1)! T(n,k)$
\begin{equation*}
(k-1)
    !T(n,k) = \frac{1}{k} \sum_{j=0} \binom{k}{j} (-1)^{j} \left( \frac{1}{2}k - j \right)^{n}
\end{equation*}
Let be $(2k-1)! T(2n, 2k)$
\begin{equation*}
(2k-1)
    !T(2n, 2k) = \frac{1}{2k} \sum_{j=0} \binom{2k}{j} (-1)^{j} (k-j)^{2n}
\end{equation*}
Since that OEIS formula defined as
\begin{equation*}
    \begin{split}
        &T(2n, 2n-2k) = \frac{1}{(2n-2k)!} \sum_{j=0} \binom{2n-2k}{j} (-1)^{j} \left( n - k - j \right)^{n} \\
        &T_{\mathrm{OEIS}} = (2(n-k) + 1)! T(2n, 2n-2k) = (2n-2k+1)! T(2n, 2n-2k)
    \end{split}
\end{equation*}
Then
\begin{equation*}
    T_{\mathrm{OEIS}} = (2n-2k+1) \sum_{j=0} \binom{2n-2k}{j} (-1)^{j} (n-k-j)^{2n}
\end{equation*}
Above is \texttt{OEISFormula2} in mathematica packageâ€”it does not work.