%! suppress = MissingLabel

\subsection{Part 1}\label{subsec:part-1}
\begin{equation}
    \begin{split}
        \binom{n}{k} = \frac{n!}{k! (n-k)!}
        &= \frac{1}{k!} \frac{1 \cdot 2 \cdot 3 \cdots (n-k) \cdot (n-k+1) \cdots n}{1 \cdot 2 \cdot 3 \cdots (n-k)} \\
        &= \frac{1}{k!} (n-k+1) (n-k+2) (n-k+3) \cdots n \\
        &= \frac{1}{k!} n (n-1) (n-2) \cdots (n-k+1) \\
        &= \frac{1}{k!} \prod_{j=1}^{k} (n-j+1) = \frac{1}{k!} \prod_{j=0}^{k-1} (n-j)
    \end{split}
\end{equation}
\begin{equation}
    \binom{n}{k} = \binom{n-1}{k} + \binom{n-1}{k-1}
\end{equation}
\begin{equation}
    \begin{split}
        \binom{n}{k}
        &= \frac{n^{\underline{k}}}{k!} = \frac{1}{k!} n (n-1) (n-2) \cdots (n-k+1) \\
        &= \frac{1}{k!} \prod_{j=1}^{k} (n-j+1) = \frac{1}{k!} \prod_{j=0}^{k-1} (n-j)
    \end{split}
\end{equation}
\begin{equation}
    \sum_{r=0}^{n} \binom{r}{c} = \binom{n+1}{c+1}
\end{equation}
\begin{equation}
    \sum_{k=0}^{n} \binom{r+k}{k} = \binom{r+n+1}{n}
\end{equation}
\begin{equation}
    \sum_{k=0}^{m} \binom{n-k}{m-k} = \binom{n+1}{m}
\end{equation}
\begin{equation}
    \sum_{k=0}^{n} \binom{n-k}{k} = f_{n+1}
\end{equation}
\begin{equation}
    k \binom{n}{k} = n \binom{n-1}{k-1}
\end{equation}
\begin{equation}
    \binom{n}{m} \binom{m}{k} = \binom{n}{k} \binom{n-k}{m-k}
\end{equation}
\begin{equation}
    \sum_{j=0}^{n} \binom{n}{j} \binom{m}{k-j} = \binom{n+m}{k}
\end{equation}

\subsection{Part2}\label{subsec:part2}
\begin{equation}
    k \binom{n}{k} = n \binom{n-1}{k-1}
\end{equation}
\begin{equation}
    \frac{k}{n} \binom{n}{k} = \binom{n-1}{k-1}
\end{equation}
\begin{equation}
    \frac{k+1}{n+1} \binom{n+1}{k+1} = \binom{n}{k}
\end{equation}
\begin{equation}
    \binom{n+1}{k+1} = \frac{n+1}{k+1} \binom{n}{k}
\end{equation}

\subsection{Part 3}\label{subsec:part-3}
\begin{equation}
    \binom{t}{r} \binom{r}{k} = \binom{t}{k} \binom{t-k}{r-k}
\end{equation}
\begin{equation}
    \binom{t}{k} \binom{t-k}{r-k} = \binom{t}{t-k} \binom{t-k}{r-k} = \binom{t}{r-k} \binom{t-r+k}{t-r}
\end{equation}
By the symmetry of binomial coefficients we get
\begin{equation}
    \binom{t}{k} \binom{t-k}{r-k} = \binom{t}{k} \binom{t-k}{t-r}
\end{equation}
\begin{equation}
    \binom{t}{k} \binom{t-k}{t-r} = \binom{t}{t-k} \binom{t-k}{t-r}
\end{equation}
\subsection{Part 4}\label{subsec:part-4}
\begin{equation}
    \binom{t}{r} \binom{r}{k} = \binom{t}{k} \binom{t-k}{r-k} = \binom{t}{t-k} \binom{t-k}{r-k} = \binom{t}{r-k} \binom{t-r+k}{t-r} = \binom{t}{r-k} \binom{t-r+k}{k}
\end{equation}