\subsection{Central factorials power identity}\label{subsec:central-factorials-power-identity}
Central factorials
\begin{equation*}
    \centralFactorial{x}{n} = x \fallingFactorial{x+\frac{n}{2}-1}{n-1} \quad
    (CentralFactorial1)
\end{equation*}
\begin{equation*}
    \centralFactorial{x}{n} = x \left( x+\frac{n}{2}-1 \right) \left( x+\frac{n}{2}-1 \right) \cdots \left (x+\frac{n}{2}-n-1 \right)
\end{equation*}
\begin{equation*}
    \centralFactorial{x}{n} = x \prod_{k=1}^{n-1} \left( x+\frac{n}{2}-k \right)
    (CentralFactorial2)
\end{equation*}
Then we have power identity given by Knuth
\begin{equation*}
    x^m = \sum_{k=1}^{m} T(m, k) \centralFactorial{x}{k} \quad
    (PowerIdentity1, PowerIdentity2)
\end{equation*}
\begin{equation*}
    x^m = \sum_{k=1}^{m} T(m, k) (x-1^2)(x-2^2)\cdots(x-k^2) = \sum_{k=1}^{m} T(m, k) \prod_{j=0}^{k} (n-j^2)
\end{equation*}
\begin{equation*}
    \mathtt{PowerProduct}(n, k) = \prod_{j=0}^{k} (n-j^2)
\end{equation*}