\subsection{Central factorial numbers}\label{subsec:central-factorial-numbers}

\begin{equation*}
(2k-1)
    !T(2n,2k) = \frac{1}{k} \sum_{j=0}^{k} (-1)^j \binom{2k}{j} (k-j)^{2n} \quad
    (CFNIdentity1)
\end{equation*}
\begin{equation*}
(2k-1)
    !T(2n,2k) = \frac{1}{k} \sum_{j=0}^{k} (-1)^{k-j} \binom{2k}{k-j} j^{2n} \quad
    (CFNIdentity2)
\end{equation*}
\begin{equation*}
(2k-1)
    !T(2n, 2k) = \frac{1}{2k} \sum_{j=0}^{2k} \binom{2k}{j} (-1)^{j} (k-j)^{2n} \quad
    (CFNIdentity3)
\end{equation*}
\begin{equation*}
    T(n,k) = \frac{1}{k!} \sum_{j=0} \binom{k}{j} (-1)^{j} \left( \frac{1}{2}k - j \right)^{n} \quad
    (CentralFactorialNumber2)
\end{equation*}
\begin{equation*}
    T(2n,2k) = 2 \sum_{j=1}^{k} (-1)^{k-j} \frac{j^{2n}}{(k-j)! (k+j)!} \quad
    (CentralFactorialNumber3)
\end{equation*}
\begin{equation*}
T(2n,2k) = \frac{1}{k (2k-1)!} \sum_{j=0}^{k} (-1)^{k-j} \binom{2k}{k-j} j^{2n} \quad
    (CentralFactorialNumber4)
\end{equation*}