\subsection{Knuth's formula - approach 3 (to be verified all)}\label{subsec:knuth's-formula---approach-3-(to-be-verified-all)}
Let be
\begin{equation*}
(2k-1)
    !T(2n, 2k) = \frac{1}{2k} \sum_{j=0}^{2k} \binom{2k}{j} (-1)^{j} (k-j)^{2n}
\end{equation*}
And
\begin{equation*}
    n^{2m-1} = \sum_{k=1}^{m} (2k-1)! T(2m,2k) \binom{n+k-1}{2k-1}
\end{equation*}
Then
\begin{equation*}
    n^{2m-1} = \sum_{k=1}^{m} \frac{1}{2k} \sum_{j=0}^{2k} \binom{2k}{j} (-1)^{j} (k-j)^{2m} \binom{n+k-1}{2k-1}
\end{equation*}
\begin{equation*}
    n^{2m-1} = \sum_{k=1}^{m} \sum_{j=0}^{2k} \frac{(-1)^{j}}{2k} \binom{n+k-1}{2k-1} \binom{2k}{j} (k-j)^{2m}
\end{equation*}
By means of binomial identity $\frac{k}{n} \binom{n}{k} = \binom{n-1}{k-1}$
\begin{equation*}
    n^{2m-1} = \sum_{k=1}^{m} \sum_{j=0}^{2k} \frac{(-1)^{j}}{2k} \frac{2k}{n+k} \binom{n+k}{2k} \binom{2k}{j} (k-j)^{2m}
\end{equation*}
Collapsing common terms we get
\begin{equation*}
    n^{2m-1} = \sum_{k=1}^{m} \sum_{j=0}^{2k} \frac{(-1)^{j}}{n+k} \binom{n+k}{2k} \binom{2k}{j} (k-j)^{2m}
\end{equation*}
By means of binomial identity $\binom{n}{m} \binom{m}{k} = \binom{n}{k} \binom{n-k}{m-k}$ we get
\begin{equation*}
    n^{2m-1} = \sum_{k=1}^{m} \sum_{j=0}^{2k} \frac{(-1)^{j}}{n+k} \binom{n+k}{j} \binom{n+k-j}{2k-j} (k-j)^{2m}
\end{equation*}
Because the symmetry of binomial coefficients $\binom{n+k}{j} = \binom{n+k}{n+k-j}$ holds, we get
\begin{equation*}
    n^{2m-1} = \sum_{k=1}^{m} \sum_{j=0}^{2k} \frac{(-1)^{j}}{n+k} \binom{n+k}{n+k-j} \binom{n+k-j}{2k-j} (k-j)^{2m}
\end{equation*}
By means of binomial identity $\binom{n}{m} \binom{m}{k} = \binom{n}{k} \binom{n-k}{m-k}$ we get
\begin{equation*}
    n^{2m-1} = \sum_{k=1}^{m} \sum_{j=0}^{2k} \frac{(-1)^{j}}{n+k} \binom{n+k}{2k-j} \binom{n-k+j}{n-k} (k-j)^{2m}
\end{equation*}