\subsection{Knuth's formula for odd power: approach 2}\label{subsec:knuth's-formula-for-odd-power-approach-2}
\begin{equation*}
    n^{2m-1} = \sum_{k=1}^{m} (2k-1)! T(2m,2k) \binom{n+k-1}{2k-1} \quad
    (OddPowerIdentity(1,2,3))
\end{equation*}
\begin{equation*}
    n^{2m-1} = \sum_{k=1}^{m} T(2m,2k) \fallingFactorial{n+k-1}{2k-1} \quad
    (OddPowerIdentity4)
\end{equation*}
Equation~\eqref{eq:knuth-general} is validated via Mathematica functions:
\textit{OddPowerIdentity1}, \textit{OddPowerIdentity2}, \textit{OddPowerIdentity3}.
Substituting $(2k-1)! T(2n,2k) = \frac{1}{k} \sum_{j=0}^{k} (-1)^{k-j} \binom{2k}{k-j} j^{2n}$ we get
\begin{equation*}
    n^{2m-1} = \sum_{k=1}^{m} \sum_{j=0}^{k} \frac{(-1)^{k-j}}{k} \binom{n+k-1}{2k-1} \binom{2k}{k-j} j^{2m} \quad
    (OddPowerIdentity21)
\end{equation*}
By means of binomial identity $\frac{k}{n} \binom{n}{k} = \binom{n-1}{k-1}$
\begin{equation*}
    n^{2m-1} = \sum_{k=1}^{m} \sum_{j=0}^{k} \frac{(-1)^{k-j}}{k} \frac{2k}{n+k} \binom{n+k}{2k} \binom{2k}{k-j} j^{2m} \quad
    (OddPowerIdentity22)
\end{equation*}
Collapsing common terms we get
\begin{equation*}
    n^{2m-1} = 2\sum_{k=1}^{m} \sum_{j=0}^{k} \frac{(-1)^{k-j}}{n+k} \binom{n+k}{2k} \binom{2k}{k-j} j^{2m} \quad
    (OddPowerIdentity23)
\end{equation*}
By means of binomial identity $\binom{n}{m} \binom{m}{k} = \binom{n}{k} \binom{n-k}{m-k}$ we get
\begin{equation*}
    n^{2m-1} = 2\sum_{k=1}^{m} \sum_{j=0}^{k} \frac{(-1)^{k-j}}{n+k} \binom{n+k}{k-j} \binom{n+j}{k+j} j^{2m} \quad
    (OddPowerIdentity24)
\end{equation*}
Because the symmetry of binomial coefficients $\binom{n+k}{k-j} = \binom{n+k}{n+k-(k-j)}$ holds, we get
\begin{equation*}
    n^{2m-1} = 2\sum_{k=1}^{m} \sum_{j=0}^{k} \frac{(-1)^{k-j}}{n+k} \binom{n+k}{n+j} \binom{n+j}{k+j} j^{2m} \quad
    (OddPowerIdentity25)
\end{equation*}
By means of binomial identity $\binom{n}{m} \binom{m}{k} = \binom{n}{k} \binom{n-k}{m-k}$ we get
\begin{equation*}
    n^{2m-1} = 2\sum_{k=1}^{m} \sum_{j=0}^{k} \frac{(-1)^{k-j}}{n+k} \binom{n+k}{k+j} \binom{n-j}{n-k} j^{2m} \quad
    (OddPowerIdentity26)
\end{equation*}