\subsection{Central factorial numbers}\label{subsec:central-factorial-numbers}
\begin{align*}
(2k-1)!T(2n,2k) &= \frac{1}{k} \sum_{j=0}^{k} (-1)^j \binom{2k}{j} (k-j)^{2n} \\
(2k-1)! T(2n,2k) &= \frac{1}{k} \sum_{j=0}^{k} (-1)^{k-j} \binom{2k}{k-j} j^{2n} \\
(2k-1)! T(2n,2k) &= \frac{1}{k} 2k! \left( \stirlingii{2n}{2k} -  \sum_{j=k+1}^{2k} (-1)^j \binom{2k}{j} (k-j)^{2n}\right) \\
\end{align*}
\begin{equation*}
    T(n,k) = \frac{1}{k!} \sum_{j=0} \binom{k}{j} (-1)^{j} \left( \frac{1}{2}k - j \right)^{n}
\end{equation*}
\begin{equation*}
(2k-1)! \cdot T(2n, 2k) = \frac{1}{2k} \sum_{j=0}^{2k} \binom{2k}{j} (-1)^{j} (k-j)^{2n}
\end{equation*}

\subsection{Knuth's formula - approach 1 (to be verified all)}\label{subsec:knuth's-formula---approach-1-(to-be-verified-all)}
\begin{equation*}
    n^{2m-1} = \sum_{k=1}^{m} (2k-1)! T(2m,2k) \binom{n+k-1}{2k-1}
\end{equation*}
Substituting $(2k-1)! T(2n,2k) = \frac{1}{k} \sum_{j=0}^{k} (-1)^{k-j} \binom{2k}{k-j} j^{2n}$ we get
\begin{equation*}
    n^{2m-1} = \sum_{k=1}^{m} \sum_{j=0}^{k} \frac{(-1)^{k-j}}{k} \binom{n+k-1}{2k-1} \binom{2k}{k-j} j^{2m}
\end{equation*}
By means of binomial identity $\frac{k}{n} \binom{n}{k} = \binom{n-1}{k-1}$
\begin{equation*}
    n^{2m-1} = \sum_{k=1}^{m} \sum_{j=0}^{k} \frac{(-1)^{k-j}}{k} \frac{2k}{n+k} \binom{n+k}{2k} \binom{2k}{k-j} j^{2m}
\end{equation*}
Collapsing common terms we get
\begin{equation*}
    n^{2m-1} = 2\sum_{k=1}^{m} \sum_{j=0}^{k} \frac{(-1)^{k-j}}{n+k} \binom{n+k}{2k} \binom{2k}{k-j} j^{2m}
\end{equation*}
By means of binomial identity $\binom{n}{m} \binom{m}{k} = \binom{n}{k} \binom{n-k}{m-k}$
\begin{equation*}
    n^{2m-1} = 2\sum_{k=1}^{m} \sum_{j=0}^{k} \frac{(-1)^{k-j}}{n+k} \binom{n+k}{k-j} \binom{n+j}{k+j} j^{2m}
\end{equation*}

